src/GetEachN.v
@@ -1,0 +1,150 @@
+Require Import List.
+Import ListNotations.
+
+Require Import Lib.
+
+Require Import Coqlib.
+
+
+(* Works as long as you pass in enough fuel *)
+(* just use the length of the list *)
+Fixpoint get_each_n' {A : Type} (fuel : nat) (tot : nat) (l : list A) : list (list A) :=
+  match l,fuel with
+  | _ :: _,S fuel' => (firstn tot l) :: get_each_n' fuel' tot (list_drop tot l)
+  | _,_ => nil
+  end.
+
+Definition get_each_n {A : Type} (tot : nat) (l : list A) :=
+  get_each_n' (length l) tot l.
+
+Lemma get_each_n'_fuel :
+  forall {A} n (l : list A) fuel tot,
+    (n >= length l)%nat ->
+    (fuel >= length l)%nat ->
+    tot <> O ->
+    get_each_n' fuel tot l = get_each_n' (length l) tot l.
+Proof.
+  induction n; intros.
+  destruct l; simpl in *; destruct fuel; try reflexivity; omega.
+  destruct l. simpl in *.
+  destruct fuel; reflexivity.
+  assert (n >= length l)%nat by (simpl in *; omega).
+  simpl. destruct tot; try omega.
+  simpl. destruct fuel; simpl in *; try omega.
+  f_equal.
+  assert (tot = O \/ tot <> O) by omega.
+  destruct H3. subst. simpl.
+  eapply IHn; eauto; omega.
+  assert (length (list_drop tot l) <= length l)%nat by (eapply list_drop_length; eauto).
+  erewrite IHn; try omega.
+  symmetry.
+  eapply IHn; omega.
+Qed.
+    
+
+Lemma get_each_n_head :
+  forall {A : Type} (l l' : list A) n,
+    n = length l ->
+    n <> O ->
+    get_each_n n (l ++ l') = [l] ++ get_each_n n l'.
+Proof.
+  induction l; intros.
+  simpl in *. congruence.
+  simpl in *.
+  destruct n; inversion H.
+  assert (n = O \/ n <> O) by omega.
+  destruct H1. subst. 
+  destruct l; simpl in H1; try omega.
+  simpl. unfold get_each_n. simpl. reflexivity.
+  unfold get_each_n. simpl.
+  rewrite firstn_app.
+  rewrite list_drop_app.
+  f_equal.
+  unfold get_each_n in IHl.
+  eapply get_each_n'_fuel; eauto.
+  
+  rewrite app_length.
+  omega.
+Qed.
+
+Lemma get_each_n'_zero :
+  forall {A} fuel (l : list A),
+    l <> nil ->
+    get_each_n' fuel O l = repeat [] fuel.
+Proof.
+  induction fuel; intros.
+  simpl. destruct l; reflexivity.
+  simpl. destruct l; try congruence.
+  erewrite IHfuel; eauto.
+Qed.
+
+
+Lemma get_each_n'_map_commutes_strong :
+  forall {A B : Type} (f : A -> B) len k l fuel n,
+    (len >= Datatypes.length l)%nat ->
+    (k >= fuel)%nat ->
+    get_each_n' fuel n (map f l) = map (map f) (get_each_n' fuel n l).
+Proof.
+  induction len; induction k; intros.
+  assert (fuel = O) by omega. subst. simpl.
+  destruct l; reflexivity.
+  destruct l; simpl in H; try omega.
+  simpl. destruct fuel; simpl; reflexivity.
+  destruct fuel; try omega.
+  destruct l; simpl; reflexivity.
+  assert (fuel = S k \/ k >= fuel)%nat by omega.
+  destruct H1. subst.
+  simpl. destruct l; simpl; auto.
+  f_equal. erewrite <- firstn_map. reflexivity.
+  replace (f a :: map f l) with (map f (a :: l)) by auto.
+  erewrite list_map_drop.
+  assert (n = O \/ n > O)%nat by omega.
+  destruct H1. subst. repeat erewrite get_each_n'_zero by (simpl; congruence).
+  eapply map_repeat_nil.
+  eapply IHlen.
+  eapply length_list_drop in H1.
+  instantiate (1 := a :: l) in H1.
+  omega. congruence.
+  instantiate (1 := k). omega.
+  eauto.
+Qed.
+
+Lemma get_each_n_map_commutes :
+  forall {A B : Type} (f : A -> B) n l,
+    get_each_n n (map f l) = map (map f) (get_each_n n l).
+Proof.
+  intros.
+  unfold get_each_n.
+  erewrite get_each_n'_map_commutes_strong.
+  erewrite map_length. reflexivity.
+  instantiate (1 := Datatypes.length l). omega.
+  instantiate (1 := Datatypes.length (map f l)). omega.
+Qed.
+
+(* Everything below is for type_stream_of_bytes *)
+Lemma get_each_n'_extra_fuel :
+  forall {A} fuel fuel' n (l : list A),
+    (fuel >= fuel')%nat ->
+    (fuel' >= Datatypes.length l)%nat ->
+    get_each_n' fuel n l = get_each_n' fuel' n l.
+Proof.
+  induction fuel; intros.
+  assert (fuel' = O) by omega.
+  subst. destruct l; simpl in *; try omega.
+  reflexivity.
+  assert (fuel' = S fuel \/ fuel >= fuel')%nat by omega.
+  destruct H1. subst. reflexivity.
+
+  destruct l; simpl.
+  simpl in *.
+  destruct fuel'; simpl; auto.
+
+  destruct fuel'. simpl in H0; omega.
+  simpl. f_equal.
+
+  simpl in H0.
+
+  (* almost there? *)
+Admitted.
+
+
