src/Lib.v
@@ -1,0 +1,188 @@
+Require Import List.
+Import ListNotations.
+
+Require Import Coqlib.
+
+
+Lemma Forall_Forall2_implies :
+  forall {A B} (P : A -> Prop) (Q R : A -> B -> Prop) (l : list A),
+    Forall P l ->
+    (forall a, P a -> forall b, Q a b -> R a b) ->
+    forall (vs : list B),
+      Forall2 Q l vs ->
+      Forall2 R l vs.
+Proof.
+  induction 1; intros.
+  inversion H0. subst.
+  econstructor. 
+  inversion H2. subst.
+  econstructor; eauto.
+Qed.
+
+(* Just like Forall2, but with 3 lists *)
+(* Good for modeling evaluation of binary operators *)
+Inductive Forall3 {A B C : Type} (TR : A -> B -> C -> Prop) : list A -> list B -> list C -> Prop :=
+| Forall3_nil :
+    Forall3 TR [] [] []
+| Forall3_cons :
+    forall x y z lx ly lz,
+      TR x y z ->
+      Forall3 TR lx ly lz ->
+      Forall3 TR (x :: lx) (y :: ly) (z :: lz).
+
+Lemma length_cons :
+  forall {A} (e : A) l,
+    Datatypes.length (e :: l) = S (Datatypes.length l).
+Proof.
+  reflexivity.
+Qed.
+
+Lemma map_cons :
+  forall {A B} (f : A -> B) (e : A) l,
+    map f (e :: l) = (f e) :: (map f l).
+Proof.
+  reflexivity.
+Qed.
+
+Lemma succ_nat_pred :
+  forall n,
+    (Z.of_nat (S n)) - 1 = Z.of_nat n.
+Proof.
+  intros.
+  repeat rewrite Nat2Z.inj_succ.
+  omega.
+Qed.
+
+Lemma Forall_app :
+  forall {A} (l1 l2 : list A) P,
+    Forall P (l1 ++ l2) <-> Forall P l1 /\ Forall P l2.
+Proof.
+  induction l1; intros; split; intros; simpl; auto.
+  destruct H. auto.
+  simpl in H. inversion H. subst.
+  rewrite IHl1 in H3.
+  destruct H3. split.
+  econstructor; eauto.
+  eauto.
+  destruct H. inversion H. econstructor; eauto.
+  rewrite IHl1. split; eauto.
+Qed.
+
+Lemma Forall_map :
+  forall {A} (l : list A) P f,
+    Forall P l ->
+    (forall x, P x -> P (f x)) ->
+    Forall P (map f l).
+Proof.
+  induction 1; intros; simpl; auto.
+Qed.
+
+Lemma firstn_map :
+  forall {A B: Type} (f : A -> B)  n l,
+    firstn n (map f l) = map f (firstn n l).
+Proof.
+  induction n; intros.
+  simpl. reflexivity.
+  simpl. destruct l; simpl. reflexivity.
+  f_equal. eapply IHn.
+Qed.
+
+Lemma map_repeat_nil :
+  forall {A B} k (f : A -> B),
+    repeat [] k = map (map f) (repeat [] k).
+Proof.
+  induction k; intros; simpl; auto.
+  f_equal. auto.
+Qed.
+
+Lemma length_list_drop :
+  forall {A} (l : list A) n,
+    (n > O)%nat ->
+    l <> nil ->
+    (Datatypes.length (list_drop n l) < Datatypes.length l)%nat.
+Proof.
+  induction l; intros.
+  destruct n; simpl; try omega; congruence.
+  simpl.
+  destruct n; try omega.
+  simpl.
+  destruct n; try solve [simpl; auto].
+  specialize (IHl (S n)).
+  assert (l = nil \/ l <> []) by (destruct l; try solve [left; congruence]; right; congruence).
+  destruct H1. subst l; simpl; auto.
+  assert (S n > O)%nat by omega.
+  eapply IHl in H2; try eapply H1. omega.
+Qed.
+
+Lemma map_injective_function :
+  forall {A B} (f : A -> B) (l : list A),
+    Forall (fun a => (forall b, f a = f b -> a = b)) l ->
+    forall l',
+      map f l = map f l' ->
+      l = l'.
+Proof.
+  induction l; intros; simpl in *.
+  destruct l'; simpl in *; try congruence; auto.
+  destruct l'; simpl in *; try congruence.
+  inversion H0.
+  inversion H. subst. eapply H5 in H2. subst.
+  f_equal.
+  eapply IHl; eauto.
+Qed.      
+
+Lemma combine_injective :
+  forall {A B : Type} (l1 : list A) (l2 : list B),
+  forall l3 l4,
+    combine l1 l2 = combine l3 l4 ->
+    (Datatypes.length l1 = Datatypes.length l2) ->
+    (Datatypes.length l3 = Datatypes.length l4) ->
+    l1 = l3 /\ l2 = l4.
+Proof.
+  induction l1; intros; simpl in *.
+  destruct l2; destruct l3; destruct l4; simpl in *; try congruence.
+  split; auto.
+  destruct l2; destruct l3; destruct l4; simpl in *; try congruence.
+  inversion H0. inversion H1. inversion H. subst. clear H H0 H1.
+  eapply IHl1 in H7; eauto. destruct H7. subst. split; auto.
+Qed.
+
+Lemma list_pair_parts_eq :
+  forall {A B : Type} (l1 l2 : list (A * B)),
+    map fst l1 = map fst l2 ->
+    map snd l1 = map snd l2 ->
+    l1 = l2.
+Proof.
+  induction l1; intros;
+    destruct l2; simpl in *; try congruence.
+  inversion H. inversion H0.
+  f_equal.
+  destruct a; destruct p; simpl in *.
+  congruence.
+  subst.
+  eapply IHl1; eauto.
+Qed.
+
+Lemma firstn_app :
+  forall {A} (l : list A) l',
+    firstn (length l) (l ++ l') = l.
+Proof.
+  induction l; intros; simpl; auto.
+  f_equal. eapply IHl.
+Qed.
+
+Lemma list_drop_app :
+  forall {A} (l : list A) l',
+    list_drop (length l) (l ++ l') = l'.
+Proof.
+  induction l; intros; simpl; auto.
+Qed.
+
+Lemma list_drop_length :
+  forall {A} (l : list A) n,
+    (length (list_drop n l) <= length l)%nat.
+Proof.
+  induction l; intros.
+  simpl. destruct n; simpl; omega.
+  simpl. destruct n; simpl. omega.
+  specialize (IHl n). omega.
+Qed.
