verif/GlobalExtends.v
@@ -1,0 +1,182 @@
+Require Import List.
+Import ListNotations.
+Require Import String.
+
+(* Borrow from CompCert *)
+Require Import Coqlib.
+Require Import Bitvectors.
+
+Require Import AST.
+Require Import Semantics.
+Require Import Utils.
+Require Import Builtins.
+Require Import BuiltinSem.
+Require Import BuiltinSyntax.
+Require Import Values.        
+Require Import Eager.
+Require Import Bitstream.
+
+
+Definition name_irrel {A : Type} (E : ident -> option A) : Prop :=
+  forall id id',
+    if ident_eq id id' then E id = E id' else True.
+
+
+Lemma name_irrel_diff_results :
+  forall {A} E id id',
+    @name_irrel A E ->
+    E id <> E id' ->
+    exists p,
+      ident_eq id id' = right p.
+Proof.
+  intros.
+  unfold name_irrel in H.
+  specialize (H id id').
+  destruct (ident_eq id id') eqn:?.
+  congruence.
+  exists n. eauto.
+Qed.
+
+
+Definition global_extends (ge GE : genv) : Prop := True.
+(* TODO *)
+(*
+Definition global_extends (ge GE : genv) : Prop :=
+  (forall id v,
+    ge id = Some v ->
+    GE id = Some v) /\
+(*  (forall TE SE expr v,
+      eager_eval_expr ge TE SE expr v ->
+      eager_eval_expr GE TE SE expr v) /\*)
+  exists l, (forall id x, ge id = Some x -> In x l) /\
+              exists l',
+                (forall id x, GE id = Some x -> In x l') /\
+                (forall x, In x l -> In x l').
+                                           
+*)
+
+Lemma global_extends_refl :
+  forall ge,
+    global_extends ge ge.
+Proof.
+Admitted.
+(*
+  unfold global_extends.
+  split. auto.
+  split. auto.
+  admit. (* TODO: we'll need to pass this in *)
+Admitted.
+*)
+(*
+Lemma global_extends_eager_eval' :
+    forall expr TE SE ge GE,
+      global_extends ge GE ->
+      forall v,
+        eager_eval_expr ge TE SE expr v ->
+        eager_eval_expr GE TE SE expr v.
+Proof.
+  intros. unfold global_extends in *.
+  destruct H. destruct H1.
+  eapply H1; eauto.
+Qed.*)
+
+Lemma global_extends_eager_eval :
+    forall expr v ge TE SE,
+      eager_eval_expr ge TE SE expr v ->
+      forall GE,
+        global_extends ge GE ->
+        eager_eval_expr GE TE SE expr v.
+Proof.
+Admitted.
+(*  intros. eapply global_extends_eager_eval'; eauto.
+Qed.*)
+
+(* Add a list to the GE that is all the things that GE contains *)
+(*
+Lemma eager_eval_expr_ident_irrel :
+  forall ge id,
+    ge id = None ->
+    (forall id' exp',
+        ge id' = Some exp' ->
+        forall id0 exp0 TE SE v,
+          eager_eval_expr ge TE SE exp' v ->
+          eager_eval_expr (extend ge id0 exp0) TE SE exp' v) ->
+    name_irrel ge ->
+    forall expr TE SE v,
+      eager_eval_expr ge TE SE expr v ->
+      forall v',
+        eager_eval_expr (extend ge id v') TE SE expr v.
+Proof. 
+  intros ge id Hnon Hnirr expr.
+  eapply Expr_ind_useful with (e := expr); intros.
+  * inversion H0. subst.
+    econstructor; eauto.
+    admit. admit.
+
+  * inversion H0. subst.
+    econstructor; eauto.
+    unfold Pl in H.
+    eapply Forall_Forall2_implies; try eapply H2; try eapply H.
+    intros. eauto.
+
+  * admit.
+
+  * admit.
+
+  * admit.
+  * admit.
+  * admit.
+  * inversion H.
+    subst. econstructor; eauto.
+    subst.
+    edestruct (@name_irrel_diff_results Expr); try eassumption; try congruence.
+    instantiate (1 := id). instantiate (1 := id0).
+    congruence.
+    eapply eager_eval_global_var. eauto.
+    unfold extend. rewrite H0.
+    eauto.
+    
+    
+Admitted.
+
+Lemma eager_eval_expr_ident_irrel_parallel :
+  forall expr ge ge' TE SE v,
+    (eager_eval_expr ge TE SE expr v -> 
+    eager_eval_expr ge' TE SE expr v) ->
+    forall id exp,
+      eager_eval_expr (extend ge id exp) TE SE expr v ->
+      eager_eval_expr (extend ge' id exp) TE SE expr v.
+Proof.
+Admitted.
+ *)
+
+Lemma global_extends_extend_r :
+  forall ge ge',
+    global_extends ge ge' ->
+    name_irrel ge ->
+    forall id exp,
+      ge id = None ->
+      global_extends ge (extend ge' id exp).
+Proof.
+Admitted.
+(*  intros.
+  unfold global_extends in *.
+  destruct H. split.
+  intros.
+  unfold extend.
+  remember H3 as Hsome.
+  clear HeqHsome.
+  eapply H in H3.
+  rewrite H3.
+  destruct (ident_eq id0 id) eqn:?; auto.
+  unfold name_irrel in *.
+  specialize (H0 id0 id).
+  rewrite Heqs in H0. congruence.
+
+  intros.
+  eapply eager_eval_expr_ident_irrel in H1; eauto.
+  eapply H2 in H3.
+  eapply eager_eval_expr_ident_irrel_parallel.
+  eapply H2. eauto.
+Qed.
+*)
